theories/ordinals/Ackermann/NNtheory.v
@@ -8,22 +8,22 @@ From hydras Require Import Compat815.
 Import NNnotations. 
 
 Lemma natNE (a b : nat) :
-  a <> b -> SysPrf NN (natToTerm a <> natToTerm b)%nn.
+  a <> b -> SysPrf NN (natToTerm a <> natToTerm b)%fol.
 Proof. 
   revert a b; 
     assert (* wlog ? *)
       (H: forall a b : nat,
-          a < b -> SysPrf NN (natToTerm a <> natToTerm b)%nn).
+          a < b -> SysPrf NN (natToTerm a <> natToTerm b)%fol).
   { induction a as [| a Hreca]; intros.
     - destruct b as [| n].
       + elim (Nat.nlt_0_r _ H).
-      + cbn; apply impE with (Succ (natToTerm n) <> Zero)%nn.
+      + cbn; apply impE with (Succ (natToTerm n) <> Zero)%fol.
         * apply cp2, impI, eqSym.
           apply Axm; right; constructor.
         * apply nn1.
     - destruct b as [| n].
       + elim (Nat.nlt_0_r _ H).
-      + cbn; apply impE with (natToTerm a <> natToTerm n)%nn.
+      + cbn; apply impE with (natToTerm a <> natToTerm n)%fol.
         * apply cp2, nn2.
         * apply Hreca; lia. 
   }
@@ -31,19 +31,19 @@ Proof.
    destruct (Nat.lt_gt_cases a b) as [H1 _]; specialize (H1 H0);
           destruct H1 as [H1 | H1]. 
   - now apply H.
-  - apply impE with (natToTerm b <> natToTerm a)%nn.
+  - apply impE with (natToTerm b <> natToTerm a)%fol.
     + apply cp2, impI, eqSym.
       apply Axm; right; constructor.
     + now apply H.
 Qed.
        
 Lemma natLE (a b : nat):
- b <= a -> SysPrf NN (~ (natToTerm a < natToTerm b))%nn.
+ b <= a -> SysPrf NN (~ (natToTerm a < natToTerm b))%fol.
 Proof.
   intros H; induction b as [| b Hrecb].
   - apply nn7.
   - cbn; apply impE with
-      (~ (natToTerm a < natToTerm b \/ natToTerm a = natToTerm b))%nn.
+      (~ (natToTerm a < natToTerm b \/ natToTerm a = natToTerm b))%fol.
   + apply cp2, nn8.
   + apply nOr, andI.
     * apply Hrecb; lia. 
@@ -52,15 +52,15 @@ Proof.
 Qed.
 
 Lemma natLT (a b : nat):
-  a < b -> SysPrf NN (natToTerm a < natToTerm b)%nn.
+  a < b -> SysPrf NN (natToTerm a < natToTerm b)%fol.
 Proof.
   intros H; eapply orE.
   - apply nn9 with (a := natToTerm b) (b := natToTerm a).
-  - apply impI; apply contradiction with (natToTerm b < natToTerm a)%nn.
+  - apply impI; apply contradiction with (natToTerm b < natToTerm a)%fol.
     + apply Axm; right; constructor.
     + now apply sysWeaken, natLE, Nat.lt_le_incl.
   - apply impI, orSys.
-    + apply contradiction with (natToTerm b = natToTerm a)%nn.
+    + apply contradiction with (natToTerm b = natToTerm a)%fol.
       * apply Axm; right; constructor.
       * apply sysWeaken, natNE.
         unfold not in |- *; intros.
@@ -69,26 +69,26 @@ Proof.
 Qed.
 
 Lemma natPlus (a b : nat):
- SysPrf NN (natToTerm a + natToTerm b = natToTerm (a + b)%nat)%nn.
+ SysPrf NN (natToTerm a + natToTerm b = natToTerm (a + b)%nat)%fol.
 Proof.
   induction b as [| b Hrecb].
   - rewrite Nat.add_comm; cbn; apply nn3. 
   - rewrite Nat.add_comm; cbn. 
-    apply eqTrans with (Succ (natToTerm a + natToTerm b))%nn.
+    apply eqTrans with (Succ (natToTerm a + natToTerm b))%fol.
     + apply nn4.
     + apply eqSucc.
       rewrite Nat.add_comm; apply Hrecb.
 Qed.
 
 Lemma natTimes (a b : nat):
- SysPrf NN (natToTerm a *natToTerm b = natToTerm (a * b)%nat)%nn.
+ SysPrf NN (natToTerm a *natToTerm b = natToTerm (a * b)%nat)%fol.
 Proof.
   - induction b as [| b Hrecb].
     + rewrite Nat.mul_comm; cbn; apply nn5.
     + rewrite Nat.mul_comm; cbn; eapply eqTrans.
       * apply nn6.
       * rewrite Nat.add_comm;
-          apply eqTrans with (natToTerm (b * a)%nat + natToTerm a)%nn.
+          apply eqTrans with (natToTerm (b * a)%nat + natToTerm a)%fol.
         -- apply eqPlus.
            ++ rewrite Nat.mul_comm; apply Hrecb.
            ++ apply eqRefl.
@@ -98,15 +98,15 @@ Qed.
 Lemma boundedLT  (m : nat) (a : Formula) (x : nat):
   (forall n : nat,
       n < m -> SysPrf NN (substF a x (natToTerm n))) ->
-  SysPrf NN (v#x < natToTerm m -> a)%nn.
+  SysPrf NN (v#x < natToTerm m -> a)%fol.
 Proof.
   revert m a x; simple induction m; intros.
   apply impI.
-  apply contradiction with (v# x < natToTerm 0)%nn.
+  apply contradiction with (v# x < natToTerm 0)%fol.
   - apply Axm; right; constructor.
   - apply sysWeaken, nn7.
   - apply impI; eapply orE.
-    + apply impE with (v#x < natToTerm (S n))%nn.
+    + apply impE with (v#x < natToTerm (S n))%fol.
       * apply sysWeaken; cbn; apply nn8.
       * apply Axm; right; constructor.
     + apply sysWeaken, H.
@@ -125,58 +125,58 @@ Qed.
 Lemma nnPlusNotNeeded (n:nat) :
  SysPrf NN
  (v#1 < natToTerm n \/ v#1 = natToTerm n ->
-  v#1 < S_ (natToTerm n))%nn.
+  v#1 < S_ (natToTerm n))%fol.
  Proof.
   induction n as [| n Hrecn].
   - cbn; apply impI, orSys. 
-    + apply contradiction with (v#1 < Zero)%nn.
+    + apply contradiction with (v#1 < Zero)%fol.
       * apply Axm; right; constructor.
       * apply sysWeaken, nn7. 
-    + rewrite <- (subFormulaId LNN (v#1 < S_ Zero)%nn 1).
+    + rewrite <- (subFormulaId LNN (v#1 < S_ Zero)%fol 1).
       apply impE with 
-        (substF (v#1 < S_ Zero)%nn 1 Zero).
+        (substF (v#1 < S_ Zero)%fol 1 Zero).
       * apply (subWithEquals LNN).
         apply eqSym.
         apply Axm; right; constructor.
       * apply sysWeaken;
-          replace (substF (v#1 < S_ Zero)%nn 1 Zero) 
+          replace (substF (v#1 < S_ Zero)%fol 1 Zero) 
           with
-          (natToTerm 0 < natToTerm 1)%nn.
+          (natToTerm 0 < natToTerm 1)%fol.
       -- apply natLT; auto.
       -- unfold LT; now rewrite (subFormulaRelation LNN).
   - cbn; apply impI, orSys.
     + apply impE with 
-        (v#1 < natToTerm n \/ v#1 = natToTerm n)%nn.
+        (v#1 < natToTerm n \/ v#1 = natToTerm n)%fol.
       * apply sysWeaken;
-          apply impTrans with (v#1 < natToTerm (S n))%nn.
+          apply impTrans with (v#1 < natToTerm (S n))%fol.
         -- apply Hrecn.
         -- apply boundedLT.
            intros n0 H. unfold Succ.
            replace
-             (substF (v#1 < (S_ (S_ (natToTerm n))))%nn
+             (substF (v#1 < (S_ (S_ (natToTerm n))))%fol
                 1 (natToTerm n0)) 
-             with (natToTerm n0 < natToTerm (S (S n)))%nn.
+             with (natToTerm n0 < natToTerm (S (S n)))%fol.
            {  apply natLT. now apply Nat.lt_lt_succ_r. }
            unfold LT; rewrite (subFormulaRelation LNN).
            cbn; rewrite (subTermNil LNN).
            ++ reflexivity.
            ++ apply closedNatToTerm.
-      * apply impE with (v#1 < S_ (natToTerm n))%nn.
+      * apply impE with (v#1 < S_ (natToTerm n))%fol.
         -- apply sysWeaken, nn8.
         -- apply Axm; right; constructor.
     + unfold Succ; rewrite <- 
         (subFormulaId LNN 
-           (v#1 <  (S_ (S_ (natToTerm n))))%nn 1).
+           (v#1 <  (S_ (S_ (natToTerm n))))%fol 1).
       apply impE with
-        (substF (v#1 < S_ (S_ (natToTerm n)))%nn 1
+        (substF (v#1 < S_ (S_ (natToTerm n)))%fol 1
            (S_ (natToTerm n))).
       * apply (subWithEquals LNN), eqSym, Axm; right; constructor. 
       * apply sysWeaken.
         replace
           (substF 
-             (v# 1 < S_ (S_ (natToTerm n)))%nn 1
+             (v# 1 < S_ (S_ (natToTerm n)))%fol 1
              (S_ (natToTerm n))) 
-          with (natToTerm (S n) <  natToTerm (S (S n)))%nn.
+          with (natToTerm (S n) <  natToTerm (S (S n)))%fol.
         { apply natLT, Nat.lt_succ_diag_r. }
         unfold LT; rewrite (subFormulaRelation LNN); cbn. 
         rewrite (subTermNil LNN).
